libcrux-ml-dsa/proofs/fstar/extraction/Libcrux_ml_dsa.Ml_dsa_44_.Neon.fst
@@ -7,7 +7,7 @@ let generate_key_pair (randomness: t_Array u8 (sz 32)) =
   let signing_key:t_Array u8 (sz 2560) = Rust_primitives.Hax.repeat 0uy (sz 2560) in
   let verification_key:t_Array u8 (sz 1312) = Rust_primitives.Hax.repeat 0uy (sz 1312) in
   let tmp0, tmp1:(t_Array u8 (sz 2560) & t_Array u8 (sz 1312)) =
-    Libcrux_ml_dsa.Ml_dsa_generic.Instantiations.Neon.generate_key_pair_v44 randomness
+    Libcrux_ml_dsa.Ml_dsa_generic.Instantiations.Neon.Ml_dsa_44_.generate_key_pair randomness
       signing_key
       verification_key
   in
@@ -28,37 +28,53 @@ let sign
       (message context: t_Slice u8)
       (randomness: t_Array u8 (sz 32))
      =
-  Libcrux_ml_dsa.Ml_dsa_generic.Instantiations.Neon.sign (sz 4) (sz 4) (sz 16) (sz 2) (sz 96)
-    (sz 17) 95232l (sz 192) (sz 768) (sz 32) (sz 39) (sz 80) (sz 576) (sz 2560) (sz 2420)
-    (Libcrux_ml_dsa.Types.impl__as_ref (sz 2560) signing_key <: t_Array u8 (sz 2560)) message
-    context randomness
+  Libcrux_ml_dsa.Ml_dsa_generic.Instantiations.Neon.Ml_dsa_44_.sign (Libcrux_ml_dsa.Types.impl__as_ref
+        (sz 2560)
+        signing_key
+      <:
+      t_Array u8 (sz 2560))
+    message
+    context
+    randomness
 
 let sign_pre_hashed_shake128
       (signing_key: Libcrux_ml_dsa.Types.t_MLDSASigningKey (sz 2560))
       (message context: t_Slice u8)
       (randomness: t_Array u8 (sz 32))
      =
-  Libcrux_ml_dsa.Ml_dsa_generic.Instantiations.Neon.sign_pre_hashed_shake128 (sz 4) (sz 4) (sz 16)
-    (sz 2) (sz 96) (sz 17) 95232l (sz 192) (sz 768) (sz 32) (sz 39) (sz 80) (sz 576) (sz 2560)
-    (sz 2420) (Libcrux_ml_dsa.Types.impl__as_ref (sz 2560) signing_key <: t_Array u8 (sz 2560))
-    message context randomness
+  Libcrux_ml_dsa.Ml_dsa_generic.Instantiations.Neon.Ml_dsa_44_.sign_pre_hashed_shake128 (Libcrux_ml_dsa.Types.impl__as_ref
+        (sz 2560)
+        signing_key
+      <:
+      t_Array u8 (sz 2560))
+    message
+    context
+    randomness
 
 let verify
       (verification_key: Libcrux_ml_dsa.Types.t_MLDSAVerificationKey (sz 1312))
       (message context: t_Slice u8)
       (signature: Libcrux_ml_dsa.Types.t_MLDSASignature (sz 2420))
      =
-  Libcrux_ml_dsa.Ml_dsa_generic.Instantiations.Neon.verify (sz 4) (sz 4) (sz 16) (sz 2420) (sz 1312)
-    (sz 17) (sz 576) 95232l 78l (sz 192) (sz 768) (sz 32) (sz 39) (sz 80)
-    (Libcrux_ml_dsa.Types.impl_2__as_ref (sz 1312) verification_key <: t_Array u8 (sz 1312)) message
-    context (Libcrux_ml_dsa.Types.impl_4__as_ref (sz 2420) signature <: t_Array u8 (sz 2420))
+  Libcrux_ml_dsa.Ml_dsa_generic.Instantiations.Neon.Ml_dsa_44_.verify (Libcrux_ml_dsa.Types.impl_2__as_ref
+        (sz 1312)
+        verification_key
+      <:
+      t_Array u8 (sz 1312))
+    message
+    context
+    (Libcrux_ml_dsa.Types.impl_4__as_ref (sz 2420) signature <: t_Array u8 (sz 2420))
 
 let verify_pre_hashed_shake128
       (verification_key: Libcrux_ml_dsa.Types.t_MLDSAVerificationKey (sz 1312))
       (message context: t_Slice u8)
       (signature: Libcrux_ml_dsa.Types.t_MLDSASignature (sz 2420))
      =
-  Libcrux_ml_dsa.Ml_dsa_generic.Instantiations.Neon.verify_pre_hashed_shake128 (sz 4) (sz 4) (sz 16)
-    (sz 2420) (sz 1312) (sz 17) (sz 576) 95232l 78l (sz 192) (sz 768) (sz 32) (sz 39) (sz 80)
-    (Libcrux_ml_dsa.Types.impl_2__as_ref (sz 1312) verification_key <: t_Array u8 (sz 1312)) message
-    context (Libcrux_ml_dsa.Types.impl_4__as_ref (sz 2420) signature <: t_Array u8 (sz 2420))
+  Libcrux_ml_dsa.Ml_dsa_generic.Instantiations.Neon.Ml_dsa_44_.verify_pre_hashed_shake128 (Libcrux_ml_dsa.Types.impl_2__as_ref
+        (sz 1312)
+        verification_key
+      <:
+      t_Array u8 (sz 1312))
+    message
+    context
+    (Libcrux_ml_dsa.Types.impl_4__as_ref (sz 2420) signature <: t_Array u8 (sz 2420))
