libcrux-ml-dsa/proofs/fstar/extraction/Libcrux_ml_dsa.Ml_dsa_65_.Portable.fst
@@ -4,84 +4,77 @@ open Core
 open FStar.Mul
 
 let generate_key_pair (randomness: t_Array u8 (sz 32)) =
-  let kp:Libcrux_ml_dsa.Types.t_MLDSAKeyPair (sz 1952) (sz 4032) =
-    {
-      Libcrux_ml_dsa.Types.f_signing_key = Libcrux_ml_dsa.Types.impl__zero (sz 4032) ();
-      Libcrux_ml_dsa.Types.f_verification_key = Libcrux_ml_dsa.Types.impl_2__zero (sz 1952) ()
-    }
-    <:
-    Libcrux_ml_dsa.Types.t_MLDSAKeyPair (sz 1952) (sz 4032)
-  in
+  let signing_key:t_Array u8 (sz 4032) = Rust_primitives.Hax.repeat 0uy (sz 4032) in
+  let verification_key:t_Array u8 (sz 1952) = Rust_primitives.Hax.repeat 0uy (sz 1952) in
   let tmp0, tmp1:(t_Array u8 (sz 4032) & t_Array u8 (sz 1952)) =
-    Libcrux_ml_dsa.Ml_dsa_generic.Instantiations.Portable.generate_key_pair_v65 randomness
-      kp.Libcrux_ml_dsa.Types.f_signing_key.Libcrux_ml_dsa.Types.f_value
-      kp.Libcrux_ml_dsa.Types.f_verification_key.Libcrux_ml_dsa.Types.f_value
+    Libcrux_ml_dsa.Ml_dsa_generic.Instantiations.Portable.Ml_dsa_65_.generate_key_pair randomness
+      signing_key
+      verification_key
   in
-  let kp:Libcrux_ml_dsa.Types.t_MLDSAKeyPair (sz 1952) (sz 4032) =
-    {
-      kp with
-      Libcrux_ml_dsa.Types.f_signing_key
-      =
-      { kp.Libcrux_ml_dsa.Types.f_signing_key with Libcrux_ml_dsa.Types.f_value = tmp0 }
-      <:
-      Libcrux_ml_dsa.Types.t_MLDSASigningKey (sz 4032)
-    }
-    <:
-    Libcrux_ml_dsa.Types.t_MLDSAKeyPair (sz 1952) (sz 4032)
-  in
-  let kp:Libcrux_ml_dsa.Types.t_MLDSAKeyPair (sz 1952) (sz 4032) =
-    {
-      kp with
-      Libcrux_ml_dsa.Types.f_verification_key
-      =
-      { kp.Libcrux_ml_dsa.Types.f_verification_key with Libcrux_ml_dsa.Types.f_value = tmp1 }
-      <:
-      Libcrux_ml_dsa.Types.t_MLDSAVerificationKey (sz 1952)
-    }
-    <:
-    Libcrux_ml_dsa.Types.t_MLDSAKeyPair (sz 1952) (sz 4032)
-  in
+  let signing_key:t_Array u8 (sz 4032) = tmp0 in
+  let verification_key:t_Array u8 (sz 1952) = tmp1 in
   let _:Prims.unit = () in
-  kp
+  {
+    Libcrux_ml_dsa.Types.f_signing_key = Libcrux_ml_dsa.Types.impl__new (sz 4032) signing_key;
+    Libcrux_ml_dsa.Types.f_verification_key
+    =
+    Libcrux_ml_dsa.Types.impl_2__new (sz 1952) verification_key
+  }
+  <:
+  Libcrux_ml_dsa.Types.t_MLDSAKeyPair (sz 1952) (sz 4032)
 
 let sign
       (signing_key: Libcrux_ml_dsa.Types.t_MLDSASigningKey (sz 4032))
       (message context: t_Slice u8)
       (randomness: t_Array u8 (sz 32))
      =
-  Libcrux_ml_dsa.Ml_dsa_generic.Instantiations.Portable.sign (sz 6) (sz 5) (sz 30) (sz 4) (sz 128)
-    (sz 19) 261888l (sz 128) (sz 768) (sz 48) (sz 49) (sz 55) (sz 640) (sz 4032) (sz 3309)
-    (Libcrux_ml_dsa.Types.impl__as_ref (sz 4032) signing_key <: t_Array u8 (sz 4032)) message
-    context randomness
+  Libcrux_ml_dsa.Ml_dsa_generic.Instantiations.Portable.Ml_dsa_65_.sign (Libcrux_ml_dsa.Types.impl__as_ref
+        (sz 4032)
+        signing_key
+      <:
+      t_Array u8 (sz 4032))
+    message
+    context
+    randomness
 
 let sign_pre_hashed_shake128
       (signing_key: Libcrux_ml_dsa.Types.t_MLDSASigningKey (sz 4032))
       (message context: t_Slice u8)
       (randomness: t_Array u8 (sz 32))
      =
-  Libcrux_ml_dsa.Ml_dsa_generic.Instantiations.Portable.sign_pre_hashed_shake128 (sz 6) (sz 5)
-    (sz 30) (sz 4) (sz 128) (sz 19) 261888l (sz 128) (sz 768) (sz 48) (sz 49) (sz 55) (sz 640)
-    (sz 4032) (sz 3309)
-    (Libcrux_ml_dsa.Types.impl__as_ref (sz 4032) signing_key <: t_Array u8 (sz 4032)) message
-    context randomness
+  Libcrux_ml_dsa.Ml_dsa_generic.Instantiations.Portable.Ml_dsa_65_.sign_pre_hashed_shake128 (Libcrux_ml_dsa.Types.impl__as_ref
+        (sz 4032)
+        signing_key
+      <:
+      t_Array u8 (sz 4032))
+    message
+    context
+    randomness
 
 let verify
       (verification_key: Libcrux_ml_dsa.Types.t_MLDSAVerificationKey (sz 1952))
       (message context: t_Slice u8)
       (signature: Libcrux_ml_dsa.Types.t_MLDSASignature (sz 3309))
      =
-  Libcrux_ml_dsa.Ml_dsa_generic.Instantiations.Portable.verify (sz 6) (sz 5) (sz 30) (sz 3309)
-    (sz 1952) (sz 19) (sz 640) 261888l 196l (sz 128) (sz 768) (sz 48) (sz 49) (sz 55)
-    (Libcrux_ml_dsa.Types.impl_2__as_ref (sz 1952) verification_key <: t_Array u8 (sz 1952)) message
-    context (Libcrux_ml_dsa.Types.impl_4__as_ref (sz 3309) signature <: t_Array u8 (sz 3309))
+  Libcrux_ml_dsa.Ml_dsa_generic.Instantiations.Portable.Ml_dsa_65_.verify (Libcrux_ml_dsa.Types.impl_2__as_ref
+        (sz 1952)
+        verification_key
+      <:
+      t_Array u8 (sz 1952))
+    message
+    context
+    (Libcrux_ml_dsa.Types.impl_4__as_ref (sz 3309) signature <: t_Array u8 (sz 3309))
 
 let verify_pre_hashed_shake128
       (verification_key: Libcrux_ml_dsa.Types.t_MLDSAVerificationKey (sz 1952))
       (message context: t_Slice u8)
       (signature: Libcrux_ml_dsa.Types.t_MLDSASignature (sz 3309))
      =
-  Libcrux_ml_dsa.Ml_dsa_generic.Instantiations.Portable.verify_pre_hashed_shake128 (sz 6) (sz 5)
-    (sz 30) (sz 3309) (sz 1952) (sz 19) (sz 640) 261888l 196l (sz 128) (sz 768) (sz 48) (sz 49)
-    (sz 55) (Libcrux_ml_dsa.Types.impl_2__as_ref (sz 1952) verification_key <: t_Array u8 (sz 1952))
-    message context
+  Libcrux_ml_dsa.Ml_dsa_generic.Instantiations.Portable.Ml_dsa_65_.verify_pre_hashed_shake128 (Libcrux_ml_dsa.Types.impl_2__as_ref
+        (sz 1952)
+        verification_key
+      <:
+      t_Array u8 (sz 1952))
+    message
+    context
     (Libcrux_ml_dsa.Types.impl_4__as_ref (sz 3309) signature <: t_Array u8 (sz 3309))
