libcrux-ml-dsa/proofs/fstar/extraction/Libcrux_ml_dsa.Ml_dsa_65_.fst
@@ -7,7 +7,7 @@ let generate_key_pair (randomness: t_Array u8 (sz 32)) =
   let signing_key:t_Array u8 (sz 4032) = Rust_primitives.Hax.repeat 0uy (sz 4032) in
   let verification_key:t_Array u8 (sz 1952) = Rust_primitives.Hax.repeat 0uy (sz 1952) in
   let tmp0, tmp1:(t_Array u8 (sz 4032) & t_Array u8 (sz 1952)) =
-    Libcrux_ml_dsa.Ml_dsa_generic.Multiplexing.generate_key_pair_v65 randomness
+    Libcrux_ml_dsa.Ml_dsa_generic.Multiplexing.Ml_dsa_65_.generate_key_pair randomness
       signing_key
       verification_key
   in
@@ -28,37 +28,53 @@ let sign
       (message context: t_Slice u8)
       (randomness: t_Array u8 (sz 32))
      =
-  Libcrux_ml_dsa.Ml_dsa_generic.Multiplexing.sign (sz 6) (sz 5) (sz 30) (sz 4) (sz 128) (sz 19)
-    261888l (sz 128) (sz 768) (sz 48) (sz 49) (sz 55) (sz 640) (sz 4032) (sz 3309)
-    (Libcrux_ml_dsa.Types.impl__as_ref (sz 4032) signing_key <: t_Array u8 (sz 4032)) message
-    context randomness
+  Libcrux_ml_dsa.Ml_dsa_generic.Multiplexing.Ml_dsa_65_.sign (Libcrux_ml_dsa.Types.impl__as_ref (sz
+          4032)
+        signing_key
+      <:
+      t_Array u8 (sz 4032))
+    message
+    context
+    randomness
 
 let sign_pre_hashed_shake128
       (signing_key: Libcrux_ml_dsa.Types.t_MLDSASigningKey (sz 4032))
       (message context: t_Slice u8)
       (randomness: t_Array u8 (sz 32))
      =
-  Libcrux_ml_dsa.Ml_dsa_generic.Multiplexing.sign_pre_hashed_shake128 (sz 6) (sz 5) (sz 30) (sz 4)
-    (sz 128) (sz 19) 261888l (sz 128) (sz 768) (sz 48) (sz 49) (sz 55) (sz 640) (sz 4032) (sz 3309)
-    (Libcrux_ml_dsa.Types.impl__as_ref (sz 4032) signing_key <: t_Array u8 (sz 4032)) message
-    context randomness
+  Libcrux_ml_dsa.Ml_dsa_generic.Multiplexing.Ml_dsa_65_.sign_pre_hashed_shake128 (Libcrux_ml_dsa.Types.impl__as_ref
+        (sz 4032)
+        signing_key
+      <:
+      t_Array u8 (sz 4032))
+    message
+    context
+    randomness
 
 let verify
       (verification_key: Libcrux_ml_dsa.Types.t_MLDSAVerificationKey (sz 1952))
       (message context: t_Slice u8)
       (signature: Libcrux_ml_dsa.Types.t_MLDSASignature (sz 3309))
      =
-  Libcrux_ml_dsa.Ml_dsa_generic.Multiplexing.verify (sz 6) (sz 5) (sz 30) (sz 3309) (sz 1952)
-    (sz 19) (sz 640) 261888l 196l (sz 128) (sz 768) (sz 48) (sz 49) (sz 55)
-    (Libcrux_ml_dsa.Types.impl_2__as_ref (sz 1952) verification_key <: t_Array u8 (sz 1952)) message
-    context (Libcrux_ml_dsa.Types.impl_4__as_ref (sz 3309) signature <: t_Array u8 (sz 3309))
+  Libcrux_ml_dsa.Ml_dsa_generic.Multiplexing.Ml_dsa_65_.verify (Libcrux_ml_dsa.Types.impl_2__as_ref (
+          sz 1952)
+        verification_key
+      <:
+      t_Array u8 (sz 1952))
+    message
+    context
+    (Libcrux_ml_dsa.Types.impl_4__as_ref (sz 3309) signature <: t_Array u8 (sz 3309))
 
 let verify_pre_hashed_shake128
       (verification_key: Libcrux_ml_dsa.Types.t_MLDSAVerificationKey (sz 1952))
       (message context: t_Slice u8)
       (signature: Libcrux_ml_dsa.Types.t_MLDSASignature (sz 3309))
      =
-  Libcrux_ml_dsa.Ml_dsa_generic.Multiplexing.verify_pre_hashed_shake128 (sz 6) (sz 5) (sz 30)
-    (sz 3309) (sz 1952) (sz 19) (sz 640) 261888l 196l (sz 128) (sz 768) (sz 48) (sz 49) (sz 55)
-    (Libcrux_ml_dsa.Types.impl_2__as_ref (sz 1952) verification_key <: t_Array u8 (sz 1952)) message
-    context (Libcrux_ml_dsa.Types.impl_4__as_ref (sz 3309) signature <: t_Array u8 (sz 3309))
+  Libcrux_ml_dsa.Ml_dsa_generic.Multiplexing.Ml_dsa_65_.verify_pre_hashed_shake128 (Libcrux_ml_dsa.Types.impl_2__as_ref
+        (sz 1952)
+        verification_key
+      <:
+      t_Array u8 (sz 1952))
+    message
+    context
+    (Libcrux_ml_dsa.Types.impl_4__as_ref (sz 3309) signature <: t_Array u8 (sz 3309))
