libcrux-ml-dsa/proofs/fstar/extraction/Libcrux_ml_dsa.Ml_dsa_87_.Portable.fst
@@ -7,7 +7,7 @@ let generate_key_pair (randomness: t_Array u8 (sz 32)) =
   let signing_key:t_Array u8 (sz 4896) = Rust_primitives.Hax.repeat 0uy (sz 4896) in
   let verification_key:t_Array u8 (sz 2592) = Rust_primitives.Hax.repeat 0uy (sz 2592) in
   let tmp0, tmp1:(t_Array u8 (sz 4896) & t_Array u8 (sz 2592)) =
-    Libcrux_ml_dsa.Ml_dsa_generic.Instantiations.Portable.generate_key_pair_v87 randomness
+    Libcrux_ml_dsa.Ml_dsa_generic.Instantiations.Portable.Ml_dsa_87_.generate_key_pair randomness
       signing_key
       verification_key
   in
@@ -28,39 +28,53 @@ let sign
       (message context: t_Slice u8)
       (randomness: t_Array u8 (sz 32))
      =
-  Libcrux_ml_dsa.Ml_dsa_generic.Instantiations.Portable.sign (sz 8) (sz 7) (sz 56) (sz 2) (sz 96)
-    (sz 19) 261888l (sz 128) (sz 1024) (sz 64) (sz 60) (sz 75) (sz 640) (sz 4896) (sz 4627)
-    (Libcrux_ml_dsa.Types.impl__as_ref (sz 4896) signing_key <: t_Array u8 (sz 4896)) message
-    context randomness
+  Libcrux_ml_dsa.Ml_dsa_generic.Instantiations.Portable.Ml_dsa_87_.sign (Libcrux_ml_dsa.Types.impl__as_ref
+        (sz 4896)
+        signing_key
+      <:
+      t_Array u8 (sz 4896))
+    message
+    context
+    randomness
 
 let sign_pre_hashed_shake128
       (signing_key: Libcrux_ml_dsa.Types.t_MLDSASigningKey (sz 4896))
       (message context: t_Slice u8)
       (randomness: t_Array u8 (sz 32))
      =
-  Libcrux_ml_dsa.Ml_dsa_generic.Instantiations.Portable.sign_pre_hashed_shake128 (sz 8) (sz 7)
-    (sz 56) (sz 2) (sz 96) (sz 19) 261888l (sz 128) (sz 1024) (sz 64) (sz 60) (sz 75) (sz 640)
-    (sz 4896) (sz 4627)
-    (Libcrux_ml_dsa.Types.impl__as_ref (sz 4896) signing_key <: t_Array u8 (sz 4896)) message
-    context randomness
+  Libcrux_ml_dsa.Ml_dsa_generic.Instantiations.Portable.Ml_dsa_87_.sign_pre_hashed_shake128 (Libcrux_ml_dsa.Types.impl__as_ref
+        (sz 4896)
+        signing_key
+      <:
+      t_Array u8 (sz 4896))
+    message
+    context
+    randomness
 
 let verify
       (verification_key: Libcrux_ml_dsa.Types.t_MLDSAVerificationKey (sz 2592))
       (message context: t_Slice u8)
       (signature: Libcrux_ml_dsa.Types.t_MLDSASignature (sz 4627))
      =
-  Libcrux_ml_dsa.Ml_dsa_generic.Instantiations.Portable.verify (sz 8) (sz 7) (sz 56) (sz 4627)
-    (sz 2592) (sz 19) (sz 640) 261888l 120l (sz 128) (sz 1024) (sz 64) (sz 60) (sz 75)
-    (Libcrux_ml_dsa.Types.impl_2__as_ref (sz 2592) verification_key <: t_Array u8 (sz 2592)) message
-    context (Libcrux_ml_dsa.Types.impl_4__as_ref (sz 4627) signature <: t_Array u8 (sz 4627))
+  Libcrux_ml_dsa.Ml_dsa_generic.Instantiations.Portable.Ml_dsa_87_.verify (Libcrux_ml_dsa.Types.impl_2__as_ref
+        (sz 2592)
+        verification_key
+      <:
+      t_Array u8 (sz 2592))
+    message
+    context
+    (Libcrux_ml_dsa.Types.impl_4__as_ref (sz 4627) signature <: t_Array u8 (sz 4627))
 
 let verify_pre_hashed_shake128
       (verification_key: Libcrux_ml_dsa.Types.t_MLDSAVerificationKey (sz 2592))
       (message context: t_Slice u8)
       (signature: Libcrux_ml_dsa.Types.t_MLDSASignature (sz 4627))
      =
-  Libcrux_ml_dsa.Ml_dsa_generic.Instantiations.Portable.verify_pre_hashed_shake128 (sz 8) (sz 7)
-    (sz 56) (sz 4627) (sz 2592) (sz 19) (sz 640) 261888l 120l (sz 128) (sz 1024) (sz 64) (sz 60)
-    (sz 75) (Libcrux_ml_dsa.Types.impl_2__as_ref (sz 2592) verification_key <: t_Array u8 (sz 2592))
-    message context
+  Libcrux_ml_dsa.Ml_dsa_generic.Instantiations.Portable.Ml_dsa_87_.verify_pre_hashed_shake128 (Libcrux_ml_dsa.Types.impl_2__as_ref
+        (sz 2592)
+        verification_key
+      <:
+      t_Array u8 (sz 2592))
+    message
+    context
     (Libcrux_ml_dsa.Types.impl_4__as_ref (sz 4627) signature <: t_Array u8 (sz 4627))
